Finish theorems, experiment with macro rules and substitutions

AnotherOne.lean
@@ -1,81 +1,195 @@
-
 import Std.Data.AssocList
-open Std
+import Std.Data.HashSet
+import Lean
+open Std Lean Elab Meta
 
-
--- Term type
 inductive TType : Type where
   | unit : String → TType
---  | bool : TType
   | arrow : TType → TType → TType
   deriving Repr, BEq, Inhabited, DecidableEq
 
-def Context := AssocList String TType
+def Ctx := AssocList String TType
 
 inductive Term : Type where
---  | true : Term
---  | false : Term
   | var : String → Term
   | abs : String → TType → Term → Term
   | app : Term → Term → Term
   deriving BEq, DecidableEq
 
+declare_syntax_cat stlc_type
+syntax:0 "Unit" ident : stlc_type
+syntax:50 stlc_type " → " stlc_type : stlc_type
+syntax:99 " ( " stlc_type " ) " : stlc_type
+partial def elabSTLCType : Syntax → MetaM Expr
+  | `(stlc_type| Unit $id:ident) => do
+    let id := mkStrLit id.getId.toString
+    mkAppM ``TType.unit #[id]
+  | `(stlc_type| $l:stlc_type → $r:stlc_type) => do
+    let l ← elabSTLCType l
+    let r ← elabSTLCType r
+    mkAppM ``TType.arrow #[l, r]
+  | `(stlc_type| ($t:stlc_type) ) => elabSTLCType t
+  | _ => throwUnsupportedSyntax
 
-inductive HasType : (ctx : Context) → Term → TType → Prop where
-  | var : ∀ tm t (name : String), ctx.find? name = some t → HasType ctx (.var name) t
+declare_syntax_cat stlc
+syntax:0 ident : stlc
+syntax:89 " λ " ident " : " stlc_type " , " stlc : stlc
+syntax:1 stlc stlc : stlc
+syntax:99 " ( " stlc " ) " : stlc
+partial def elabSTLC : Syntax → MetaM Expr
+  | `(stlc| $id:ident ) => mkAppM ``Term.var  #[mkStrLit id.getId.toString]
+  | `(stlc| λ $id:ident : $t:stlc_type , $tm:stlc) => do
+    let id := mkStrLit id.getId.toString
+    let t ← elabSTLCType t
+    let tm ← elabSTLC tm
+    mkAppM ``Term.abs #[id, t, tm]
+  | `(stlc| $funct:stlc $argt:stlc) => do
+    let funct ← elabSTLC funct
+    let argt ← elabSTLC argt
+    mkAppM ``Term.app #[funct, argt]
+  | `(stlc| ($tm:stlc)) => elabSTLC tm
+  | `($tk) => withRef tk (throwError "Error HEre")
+
+elab "⟪" tm:stlc "⟫" : term => elabSTLC tm
+
+inductive HasType : (ctx : Ctx) → Term → TType → Prop where
+  | var : ∀ t (name : String), ctx.find? name = some t → HasType ctx (.var name) t
   | abs : ∀ (name : String) TArg TBody tmBody,
-          HasType (ctx.insert name Targ) tmBody TBody
+          HasType (ctx.insert name TArg) tmBody TBody
         → HasType ctx (.abs name TArg tmBody) (.arrow TArg TBody)
   | app : ∀ t₁ t₂ tm₁ tm₂,
           HasType ctx tm₁ (.arrow t₁ t₂)
-        → HasType ctx tm₂ t₂
-        → HasType ctx (.app tm₁ tm₂) t2
+        → HasType ctx tm₂ t₁
+        → HasType ctx (.app tm₁ tm₂) t₂
 
-
-
-
-def typecheck : (ctx : Context) → (tm : Term) → Option TType
---  | Term.true, ctx => .found .bool (.true Term.true rfl)
---  | Term.false, ctx => .found .bool (.false Term.false rfl)
+def typecheck : (ctx : Ctx) → (tm : Term) → Option TType
   | ctx, Term.var name => ctx.find? name
-  | ctx, Term.abs name TArg tmBody => 
-    let ctx₂ := ctx.insert name TArg 
+  | ctx, Term.abs name TArg tmBody =>
+    let ctx₂ := ctx.insert name TArg
     match typecheck ctx₂ tmBody with
       | .some TBody => .some (.arrow TArg TBody)
       | _ => .none
   | ctx, Term.app tm₁ tm₂ =>
-    match (typecheck ctx tm₁, typecheck ctx tm₂) with
-      | (.some (.arrow T₁₁ T₁₂), .some T₂) → 
-        if (T₁₁ = T₂) then .some T₁₂ else .none 
-      | (_, _) => .none
-  -- | Term.abs name t₁ tm₁, ctx₁ =>
-  --   let ctx₂ := ctx₁.insert name t₁
-  --   match tm₁.typecheck ctx₂ with
-  --   | .found t₂ tm₂ =>
-  --     .found (.arrow t₁ t₂) (@WTTerm.abs ctx₁ tm₁ t₂ ctx₂ (Term.abs name t₁ tm₁) name t₁ rfl rfl tm₂)
-  --   | .unknown => .unknown
-  -- | Term.app tm₁ tm₂, ctx =>
-  --   match (tm₁, tm₁.typecheck ctx, tm₂.typecheck ctx) with
-  --   | (.abs name t' tm', .found (.arrow t₁ t₂) tm₂₁, .found t₃ tm₂₂) =>
-  --     -- (swapEqType ctx t₃ t₁ tm₂₂ h)
-  --     if h : (t₃ = t₁) ∧ (tm₁ = .abs name t₁ tm') then
-  --       .found t₂ (.app t₁ t₂ (Term.app tm₁ tm₂) tm₁ tm₂ name tm' (by
-  --         cases h <;> rename_i teq tabs
-  --         rewrite [tabs]
-  --         rfl
-  --       ) tm₂₁ (by
-  --         cases h <;> rename_i teq tabs
-  --         rewrite [← teq]
-  --         exact tm₂₂
-  --       ) rfl)
-  --     else .unknown
-  --   | _ => .unknown
+      match (typecheck ctx tm₁, typecheck ctx tm₂) with
+        | (.some (.arrow T₁₁ T₁₂), .some T₂) =>
+          if (T₁₁ = T₂) then .some T₁₂ else .none
+        | (_, _) => .none
+
+theorem Prod.eq_split : (a, b) = (c, d) → a = c ∧ b = d := by
+  intro h; cases h
+  constructor <;> rfl
+
+theorem If.ttype_decided {a b t t' : TType}
+  : (Q : ((if a = b then Option.some t else Option.none) = Option.some t'))
+  → a = b /\ t = t' := by
+  split <;> intros
+  · constructor
+    · assumption
+    · rename_i l r; injection r; assumption
+  · contradiction
+
+theorem typecheck_sound (ctx: Ctx) (tm : Term) (t : TType)
+  : (typecheck ctx tm = .some t) → HasType ctx tm t := by
+  induction tm generalizing ctx t with
+  | var name =>
+    simp [typecheck]; intro hfind
+    exact .var t name hfind
+  | abs name argₜ tm hind =>
+    simp [typecheck]; split
+    · rename_i P t' R
+      intro hteq; injection hteq with hteq; rewrite [← hteq]; clear hteq
+      exact .abs name argₜ t' tm (hind (AssocList.insert ctx name argₜ) t' R)
+    · intros; contradiction
+  | app tm₁ tm₂ hind₁ hind₂ =>
+    simp [typecheck]; split
+    · rename_i t₁₁ t₁₂ t₂ hp
+      intro hq; cases Prod.eq_split hp
+      · rename_i hterm₁type hterm₂type
+        let abstype := TType.arrow t₁₁ t₁₂
+        have ht₁ := hind₁ ctx abstype hterm₁type
+        have ht₂ := hind₂ ctx t₂ hterm₂type
+        cases If.ttype_decided hq
+        · rename_i hteq₁ hteq₂
+          rw [← hteq₂]; rw [← hteq₁] at ht₂
+          exact .app t₁₁ t₁₂ tm₁ tm₂ ht₁ ht₂
+    · intro; contradiction
+
+
+theorem typecheck_complete (ctx : Ctx) (tm : Term) (t : TType)
+  : HasType ctx tm t → typecheck ctx tm = .some t := by
+  intros hhty
+  induction hhty with
+  | var t name hfind =>
+    simp [typecheck]; rw [hfind]
+  | abs name argₜ bodyₜ body hht hbodytck =>
+    simp [typecheck]; split
+    · rename_i t' hargtck
+      simp
+      rewrite [hbodytck] at hargtck
+      injection hargtck
+      rename_i eq; rw [eq]
+    · rename_i htof
+      have hf := htof bodyₜ hbodytck
+      contradiction
+  | app argₜ bodyₜ funcₜₘ argₜₘ hhtbody hhtarg htck_func htck_arg =>
+    simp[typecheck]; split
+    · rename_i t₁₁ t₁₂ t₂ hp
+      simp_all
+      cases hp
+      · rename_i hargbodyt _ -- hargt
+        cases hargbodyt
+        simp [*] at *
+        rename_i hteq
+        rw [hteq]
+        simp
+    · simp_all
+      rename_i prod fst snd hprod happ
+      simp_all
+      cases happ
+      · rename_i hfstt hsndt
+        have fstEq := Eq.symm hfstt
+        have sndEq := Eq.symm hsndt
+        exact (hprod argₜ bodyₜ argₜ fstEq sndEq)
+
+syntax "[ " ident " := " stlc "] " stlc : term
+
+#print List
+
+def HashSet.joinList (h₁ : HashSet String) (l : List String) : HashSet String := match l with
+  | .nil => h₁
+  | .cons s xs => joinList (h₁.insert s) xs
+
+
+def HashSet.union (h₁ : HashSet String) (h₂ : HashSet String) : HashSet String 
+  := HashSet.joinList h₁ (h₂.toList)
+
+
+def Term.freeVars : (tm : Term) → (bound : HashSet String) → (acc : HashSet String) → HashSet String
+  | (.var name), bound, acc => if (bound.contains name) then acc else acc.insert name
+  | (.abs name _ body), bound, acc => freeVars body (bound.insert name) acc
+  | (.app tm₁ tm₂), bound, acc => 
+      HashSet.union (freeVars tm₁ bound acc) (freeVars tm₂ bound acc)
+
+def freshVarHelper (freeVars: List String) (acc : String) → (acc : )
+
+def freshVar (freeVars : HashSet String) : (∃ s, (freeVars.contains s) = false) := match (
+
+
+syntax " [ " ident " := " term " ] " term : term
+
+def Term.subst (name : String) : (src : Term) → (into : Term) → Term
+  -- | src@(.var n), into => if (name = n) then into else src
+  -- | src@(.abs n argT body) => if (name = n) then src else (.abs n argT )
+  | src, _ => src
+
+def 
+
+macro_rules
+  | `([ $name:ident := $into:term ] $src:term) => do
+    let name := quote name.getId.toString
+    `(Term.subst $name $src $into)
 
 
 
 
-#print typecheck
-
-
-def typecheck_correct (ctx: Context) (tm : Term) (t : TType) : (typecheck ctx tm = .some t) → HasType ctx tm t := by sorry
-
+#reduce [a := ⟪ b ⟫] ⟪ c ⟫
