ArbitraryLetters.lean
@@ -8,24 +8,121 @@ inductive TType : Type where
   | arrow : TType → TType → TType
   deriving Repr, BEq, Inhabited, DecidableEq
 
-def Context := AssocList String TType
+abbrev Context := AssocList String TType
 
 inductive Term : Type where
   | var : String → Term
   | abs : String → TType → Term → Term
   | app : Term → Term → Term
 
+#print AssocList
+
+inductive CtxKeyValueExist :  (key : String) → (value : TType) → (ctx : Context) → Prop where
+  | Here : CtxKeyValueExist key value (AssocList.cons key value ctxs)
+  | There : (later : CtxKeyValueExist key value ctxs)
+          → CtxKeyValueExist key value (AssocList.cons key' value' ctxs)
+
+inductive CtxKeyExists : (key: String) → (ctx : Context) → Prop where
+  | Here : CtxKeyExists key (AssocList.cons key value ctxs)
+  | There : (later : CtxKeyExists key ctxs)
+          → CtxKeyExists key (AssocList.cons key' value' ctxs)
+
+#print Decidable
+
+instance (name: String) (ctx: Context) : Decidable (CtxKeyExists name ctx) := by
+  induction ctx
+  constructor
+  intro bad
+  cases bad
+  
+  rename_i name' value' xs Ih
+  cases Ih with
+  | isTrue cke => cases cke
+  | isFalse cke => sorry
+
+  sorry
+  exact (.isTrue (.There Ih))
+
+
+inductive Maybe (p : α → Sort u) where
+  | found : (a : α) → p a → Maybe p
+  | unknown
+
+
+inductive InContextType (name: String) (ctx: Context): Prop where
+  | res : (t: TType) → CtxKeyValueExist name t ctx → InContextType name ctx
+
+
+inductive OptionP (α : Prop) : Prop where
+  | some (val : α) : OptionP α
+  | none : OptionP α
+
+
+def OptionP.bind : OptionP α → (α → OptionP β) → OptionP β
+  | .some a, f => f a
+  | .none, f => .none
+
+
+
+def Context.existsPair  (ctx : Context) (name: String) (type : TType) : OptionP (CtxKeyValueExist name type ctx) := match ctx with
+  | .nil => .none
+  | .cons n t xs => if h : (n = name) ∧ (t = type) then .some (by (
+    cases h
+    rename_i eq₁ eq₂
+    rewrite [eq₁, eq₂]
+    exact .Here
+  )) else match existsPair xs name type with
+    | .some x => .some (.There x)
+    | .none => .none
+    
+def Context.existsKey  (ctx : Context) (name: String) : OptionP (CtxKeyExists name ctx) := match ctx with
+  | .nil => .none
+  | .cons n t xs => if h : (n = name) then .some (by (
+    rewrite [h]
+    exact .Here
+  )) else match existsKey xs name with
+    | .some x => .some (.There x)
+    | .none => .none
+
+
+  
+  
+def Context.getValue (ctx: Context) (name: String) (keyExists: CtxKeyExists name ctx) 
+: ∃ t: TType, CtxKeyValueExist name t ctx := by
+  induction ctx
+  cases keyExists
+  rename_i name' v xs IH 
+  cases keyExists with
+  | Here => exists v; exact .Here
+  | There laterKey => 
+    have ET := IH laterKey
+    cases ET
+    rename_i t laterPair
+    exists t
+    exact .There (laterPair)
+  
+
+def Context.getValue? (ctx: Context) (name: String) : OptionP (InContextType name ctx) := match ctx with
+  | .nil => .none
+  | .cons n t xs => if h : (n = name) then .some (by (
+    exists t
+    rewrite [h]
+    exact .Here
+  )) else match getValue? xs name with
+    | .some EtP => by
+      cases EtP
+      rename_i rt later
+      constructor
+      exists rt
+      exact .There later
+    | .none => .none
+
 inductive WTTerm : (ctx : Context) → TType → Type where
-  | var : ∀ t (name : String), (ctx.find? name = some t) → WTTerm ctx t
+  | var : ∀ t (name : String), CtxKeyValueExist name t ctx → WTTerm ctx t
   | abs : ∀ t₂, (name : String) → (t₁ : TType) → (body : WTTerm (ctx.insert name t₁) t₂) → WTTerm ctx (.arrow t₁ t₂)
   | app : ∀ t₁ t₂, WTTerm ctx (.arrow t₁ t₂) → WTTerm ctx t₁ → WTTerm ctx t₂
 
-inductive Maybe (p : α → Type) where
-  | found : (a : α) → p a → Maybe p
-  | unknown
   
-
-#print Decidable
 
 def swapEqType (ctx : Context) (t₁ t₂ : TType) (tm : WTTerm ctx t₁) : (t₁ = t₂) → WTTerm ctx t₂ := by 
   intros A
@@ -39,11 +136,16 @@ def WTTerm_to_Term (ctx: Context) (t : TType) : (WTTerm ctx t) -> Term
   | .app t₁ t₂ l r => .app (WTTerm_to_Term ctx (.arrow t₁ t₂) l) (WTTerm_to_Term ctx t₁ r)
 
 
+  -- | Term.var name , ctx=> match ctx.getValue? name with
+  --   | .some ⟨e, z⟩ => (by sorry) --.found t (.var t name contextType)
+  --   | .none => .unknown
 
 def Term.typecheck : (tm : Term) → (ctx : Context) → Maybe (WTTerm ctx)
-  | Term.var name , ctx=> match contextType : ctx.find? name with
-    | some t => .found t (.var t name contextType)
-    | none => .unknown
+  | Term.var name , ctx=> by 
+    have kek := ctx.getValue? name 
+    cases kek
+
+
   | Term.abs name t₁ tm₁, ctx₁ =>
     let ctx₂ := ctx₁.insert name t₁
     match tm₁.typecheck ctx₂ with
@@ -56,9 +158,9 @@ def Term.typecheck : (tm : Term) → (ctx : Context) → Maybe (WTTerm ctx)
       else .unknown
     | _ => .unknown
 
-#print HEq
 
-def correct2 (ctx: Context) (tm : Term) (t : TType) (wtt : WTTerm ctx t): (tm = WTTerm_to_Term ctx t wtt) → Term.typecheck tm ctx = (.found t wtt) := by
+def correct2 (ctx: Context) (tm : Term) (t : TType) (wtt : WTTerm ctx t)
+  : (tm = WTTerm_to_Term ctx t wtt) → Term.typecheck tm ctx = (.found t wtt) := by
   intros A
   induction t generalizing tm ctx
   cases wtt
@@ -72,9 +174,10 @@ def correct2 (ctx: Context) (tm : Term) (t : TType) (wtt : WTTerm ctx t): (tm = 
   simp
   constructor; exact Q
   rewrite [Q]
-  
 
-  have E : HEq (WTTerm.var t name f) (WTTerm.var (TType.unit type) name f) 
+
+
+
   
   
   
