again.lean
@@ -1,0 +1,186 @@
+import Std.Data.AssocList
+open Std
+
+
+-- Term type
+inductive TType : Type where
+  | unit : String → TType
+  | arrow : TType → TType → TType
+  deriving Repr, BEq, Inhabited, DecidableEq
+
+abbrev Context := (String → TType)
+
+inductive Term : Type where
+  | var : String → Term
+  | abs : String → TType → Term → Term
+  | app : Term → Term → Term
+
+#print AssocList
+
+def Context.insert (name: String) (t : TType) (ctx : Context) := fun s => if (s = name) then t else (ctx name)
+
+inductive CtxKeyValueExist :  (key : String) → (value : TType) → (ctx : Context) → Prop where
+  | Here : CtxKeyValueExist key value (AssocList.cons key value ctxs)
+  | There : (later : CtxKeyValueExist key value ctxs)
+          → CtxKeyValueExist key value (AssocList.cons key' value' ctxs)
+
+inductive CtxKeyExists : (key: String) → (ctx : Context) → Prop where
+  | Here : CtxKeyExists key (AssocList.cons key value ctxs)
+  | There : (later : CtxKeyExists key ctxs)
+          → CtxKeyExists key (AssocList.cons key' value' ctxs)
+
+#print Decidable
+
+instance (name: String) (ctx: Context) : Decidable (CtxKeyExists name ctx) := by
+  induction ctx
+  constructor
+  intro bad
+  cases bad
+  
+  rename_i name' value' xs Ih
+  cases Ih with
+  | isTrue cke => cases cke
+  | isFalse cke => sorry
+
+  sorry
+  exact (.isTrue (.There Ih))
+
+
+inductive Maybe (p : α → Sort u) where
+  | found : (a : α) → p a → Maybe p
+  | unknown
+
+
+inductive InContextType (name: String) (ctx: Context): Prop where
+  | res : (t: TType) → (t ≠ .unit "unknown") → (ctx name = t) → InContextType name ctx
+
+
+inductive OptionP (α : Prop) : Prop where
+  | some (val : α) : OptionP α
+  | none : OptionP α
+
+def OptionP.bind : OptionP α → (α → OptionP β) → OptionP β
+  | .some a, f => f a
+  | .none, f => .none
+
+
+
+def Context.existsPair  (ctx : Context) (name: String) (type : TType) : OptionP (CtxKeyValueExist name type ctx) := match ctx with
+  | .nil => .none
+  | .cons n t xs => if h : (n = name) ∧ (t = type) then .some (by (
+    cases h
+    rename_i eq₁ eq₂
+    rewrite [eq₁, eq₂]
+    exact .Here
+  )) else match existsPair xs name type with
+    | .some x => .some (.There x)
+    | .none => .none
+    
+def Context.existsKey  (ctx : Context) (name: String) : OptionP (CtxKeyExists name ctx) := match ctx with
+  | .nil => .none
+  | .cons n t xs => if h : (n = name) then .some (by (
+    rewrite [h]
+    exact .Here
+  )) else match existsKey xs name with
+    | .some x => .some (.There x)
+    | .none => .none
+
+
+  
+  
+def Context.getValue (ctx: Context) (name: String) (keyExists: CtxKeyExists name ctx) 
+: ∃ t: TType, CtxKeyValueExist name t ctx := by
+  induction ctx
+  cases keyExists
+  rename_i name' v xs IH 
+  cases keyExists with
+  | Here => exists v; exact .Here
+  | There laterKey => 
+    have ET := IH laterKey
+    cases ET
+    rename_i t laterPair
+    exists t
+    exact .There (laterPair)
+  
+
+def Context.getValue? (ctx: Context) (name: String) : OptionP (InContextType name ctx) 
+  := if h : (ctx name = .unit "undefined") then .none else by
+    have kek : InContextType name ctx := .res (ctx name) h (rfl)
+
+inductive WTTerm : (ctx : Context) → TType → Type where
+  | var : ∀ t (name : String), (ctx name = t) /\ (ctx name ≠ .unit "unknown") → WTTerm ctx t
+  | abs : ∀ t₂, (name : String) → (t₁ : TType) → (body : WTTerm (ctx.insert name t₁) t₂) → WTTerm ctx (.arrow t₁ t₂)
+  | app : ∀ t₁ t₂, WTTerm ctx (.arrow t₁ t₂) → WTTerm ctx t₁ → WTTerm ctx t₂
+
+  
+
+def swapEqType (ctx : Context) (t₁ t₂ : TType) (tm : WTTerm ctx t₁) : (t₁ = t₂) → WTTerm ctx t₂ := by 
+  intros A
+  rewrite [← A]
+  exact tm
+
+
+def WTTerm_to_Term (ctx: Context) (t : TType) : (WTTerm ctx t) -> Term 
+  | .var type name _ => .var name
+  | .abs t₂ name t₁ body => .abs name t₁ (WTTerm_to_Term (ctx.insert name t₁) t₂ body)
+  | .app t₁ t₂ l r => .app (WTTerm_to_Term ctx (.arrow t₁ t₂) l) (WTTerm_to_Term ctx t₁ r)
+
+
+  -- | Term.var name , ctx=> match ctx.getValue? name with
+  --   | .some ⟨e, z⟩ => (by sorry) --.found t (.var t name contextType)
+  --   | .none => .unknown
+
+def Term.typecheck : (tm : Term) → (ctx : Context) → Maybe (WTTerm ctx)
+  | Term.var name , ctx=> if h : (ctx name = .unit "unknown") then .unknown
+      else .found (ctx name) (.var (ctx name) name (by constructor; rfl; assumption))
+
+  | Term.abs name t₁ tm₁, ctx₁ =>
+    let ctx₂ := ctx₁.insert name t₁
+    match tm₁.typecheck ctx₂ with
+    | .found t₂ tm₂ => .found (.arrow t₁ t₂) (.abs t₂ name t₁ tm₂)
+    | .unknown => .unknown
+  | Term.app tm₁ tm₂, ctx =>
+    match (tm₁.typecheck ctx, tm₂.typecheck ctx) with
+    | (.found (.arrow t₁ t₂) tm₂₁, .found t₃ tm₂₂) =>
+      if h : (t₃ = t₁) then .found t₂ (.app t₁ t₂ tm₂₁ (swapEqType ctx t₃ t₁ tm₂₂ h))
+      else .unknown
+    | _ => .unknown
+
+def Term.inferType (tm : Term) (ctx : Context) : Option (TType) := match Term.typecheck tm ctx with
+  | .found t tm => .some t
+  | .unknown => .none
+
+def emptyContext : Context := fun s => .unit "unknown"
+
+#reduce Term.inferType ((.var "x")) (Context.insert ("x") (.arrow (.unit "a") (.unit "b")) (Context.insert "y" (.unit "a") emptyContext))
+#reduce Term.inferType ((.var "y")) (Context.insert ("x") (.arrow (.unit "a") (.unit "b")) (Context.insert "y" (.unit "a") emptyContext))
+#reduce Term.inferType (.app (.var "x") (.var "y")) (Context.insert ("x") (.arrow (.unit "a") (.unit "b")) (Context.insert "y" (.unit "a") emptyContext))
+
+def correct2 (ctx: Context) (tm : Term) (t : TType) (wtt : WTTerm ctx t)
+  : (tm = WTTerm_to_Term ctx t wtt) → Term.inferType tm ctx = (.some t) := by
+  intros A
+  induction tm generalizing t ctx
+  cases wtt
+  simp [WTTerm_to_Term, Term.inferType, Term.typecheck]
+  rename_i type name f
+  
+
+
+
+  
+
+
+
+
+
+
+  
+  
+  
+
+  
+  
+
+
+
+
